src/dafny/utils/SeqOfSets.dfy
@@ -12,10 +12,14 @@
  * under the License.
  */
 
+
+include "MiscTypes.dfy"
 /** 
   * Provides seqeuence of sets.
   */
 module SeqOfSets {
+
+  import opened MiscTypes
 
   /**
     *   Union of a seq of sets.
@@ -43,6 +47,14 @@ module SeqOfSets {
     forall k:: 0 <= k < |xs| ==> xs[k] != {}
   }
 
+  lemma AllNonEmptySubset<T>(r1: seq<set<T>>, r2: seq<set<T>>)
+    requires AllNonEmpty(r1)
+    requires AllNonEmpty(r2)
+    ensures AllNonEmpty(r1 + r2)
+  {
+
+  }
+
   predicate DisjointAnyTwo<T>(xs: seq<set<T>>)
   {
     forall k, k':: 0 <= k < k' < |xs| ==> xs[k] * xs[k'] == {}
@@ -53,13 +65,21 @@ module SeqOfSets {
     SetU(xs) == set z {:nowarn} | 0 <= z < n
   }
 
+  lemma EmptySubsetIntersection<T>(a: set<T>, b: set<T>, c: set<T>, d: set<T>)
+    requires a * b == {}
+    requires c <= a && d <= b
+    ensures c * d == {}
+  {
+  }
+
   /**
     *   Every value in a class is less than n.
     *   Every 0 <= k < n is is in SetU(xs)
     */
   lemma AllBoundedBy(xs: seq<set<nat>>, n: nat)
     requires SetN(xs, n)
-    ensures forall k, e:: k in xs ==> e in k ==> 0 <= e < n
+    ensures forall k, e:: k in xs && e in k ==> 0 <= e < n
+    ensures forall k, e:: 0 <= k < |xs| &&  e in xs[k] ==> 0 <= e < n
     ensures forall e:: 0 <= e < n <==> e in SetU(xs)
   { //  Thanks Dafny
   }
@@ -336,6 +356,60 @@ module SeqOfSets {
       if f(xs[0]) then (r.0 + {xs[0]}, r.1)
       else
         (r.0, r.1 + {xs[0]})
+  }
+
+  /**
+    *   Flattening a seq of disjoint sets yield 
+    *   a set of disjoint sets.
+    */
+  lemma NonFlatDisjointImpliesFlatDisjoint(r: seq<seq<set<nat>>>, r': seq<set<nat>>)
+    requires r' == Flatten(r)
+    requires forall i, i':: 0 <= i < i' < |r| ==> SetU(r[i]) * SetU(r[i']) == {}
+    requires forall i:: 0 <= i < |r| ==> DisjointAnyTwo(r[i])
+    ensures DisjointAnyTwo(Flatten(r))
+  {
+    forall i, i' | 0 <= i < i' < |r'|
+      ensures r'[i] * r'[i'] == {}
+    {
+      var (i1, k1) := UnFlatIndex(r, r', i);
+      var (i2, k2) := UnFlatIndex(r, r', i');
+      FlatDistinctImpliesUnFlatDistinct(r, r', i, i');
+    }
+  }
+
+  /**
+    *   Flatten preserves SetU.
+    */
+  lemma FlattenPreservesSetU(xs: seq<set<nat>>, r: seq<seq<set<nat>>>)
+    requires |xs| == |r|
+    requires forall i:: 0 <= i < |r| ==> SetU(r[i]) == xs[i]
+    ensures SetU(Flatten(r)) == SetU(xs)
+  {
+    if |xs| == 0 {
+      //  Thanks Dafny
+    } else {
+      calc == {
+        SetU(Flatten(r));
+        SetU(r[0] + Flatten(r[1..]));
+        { DistribUnion(r[0], Flatten(r[1..])); }
+        SetU(r[0]) + SetU(Flatten(r[1..]));
+        xs[0] + SetU(Flatten(r[1..]));
+        { FlattenPreservesSetU(xs[1..], r[1..]); }
+        xs[0] + SetU(xs[1..]);
+      }
+    }
+  }
+
+  /**
+    *   Flattening all non-empty sets preserves all non-empty.
+    */
+  lemma FlattenAllNonEmpty(r: seq<seq<set<nat>>>, n: nat)
+    requires forall i:: 0 <= i < |r| ==> AllNonEmpty(r[i])
+    requires forall i, k:: 0 <= i < |r| && 0 <= k < |r[i]| ==> forall x:: x in r[i][k] ==> x < n
+    ensures forall i:: i in Flatten(r) ==> i != {}
+    ensures AllNonEmpty(Flatten(r))
+    ensures forall i:: i in Flatten(r) ==> forall x:: x in i ==> x < n
+  { // Thanks Dafny
   }
 
 }
